ulib/FStar.Tactics.Derived.fst
@@ -528,6 +528,9 @@ let rec revert_all (bs:binders) : Tac unit =
 (* Some syntax utility functions *)
 let bv_to_term (bv : bv) : Tac term = pack (Tv_Var bv)
 let binder_to_term (b : binder) : Tac term = let bv, _ = inspect_binder b in bv_to_term bv
+let name_of_binder (b:binder) : Tac string =
+  let bv, _ = inspect_binder b in
+  bv_ppname bv
 
 // Cannot define this inside `assumption` due to #1091
 private
